LeanScratch.lean
@@ -21,6 +21,7 @@ import LeanScratch.LocallyNameless.STLC.Typing
 
 import LeanScratch.PCF.Basic
 import LeanScratch.PCF.Properties
+import LeanScratch.PCF.SmallStep
 import LeanScratch.PCF.BigStep
 import LeanScratch.PCF.Semantics
 
